\documentclass[10pt]{article}
\usepackage[utf8]{inputenc}
\usepackage{amscd}
\usepackage{amsmath}
\usepackage{amssymb}
\usepackage{amsthm}
\usepackage{listings}
\usepackage{enumerate}

\textwidth=15cm \textheight=22cm \topmargin=0.5cm \oddsidemargin=0.5cm \evensidemargin=0.5cm

\newcommand{\sk}{\vskip 10mm}
\newcommand{\bb}[1]{\mathbb{#1}}
\newcommand{\ra}{\rightarrow}

\theoremstyle{plain}
\newtheorem{problem}{Problem}
\newtheorem{lemma}{Lemma}[problem]

\theoremstyle{remark}
\newtheorem{tpart}{}[problem]
\newtheorem*{ppart}{}

\begin{document}

\begin{problem}[3.1.3] %1
  
\end{problem}

\begin{proof}
  Let $a,b\in G$. Then $\text{Inn}(ab)=\phi_{ab}$. For any $g\in G$ we have
  \[\phi_{ab}(g)=abgb^{-1}a^{-1}=a\phi_b(g)a^{-1}=\phi_a\circ\phi_b(g)\]
  Which implies that $\phi_{ab}=\phi_a\circ\phi_b=\text{Inn}(a)\circ\text{Inn}(b)$
  completing the proof that $\text{Inn}$ is a group homomorphism.

  Next, for an element $a\in G$ to be in the kernel of $\text{Inn}$
  it is required to have $\phi_a(g)=g$. Then
  $gag^{-1}=a$ which by cancellation we get $ga=ag$ for all $g\in G$.
  Therefore the kernel of $\text{Inn}$ is $Z(G)$.

  Finally let $\phi_a\in\text{Inn}(G)$ and $\varphi\in\text{Aut}(G)$. Then
  the function $\varphi\circ\phi_a\circ\varphi^{-1}$ for an element $g\in G$ is
  \[ \varphi\circ\phi_a\circ\varphi^{-1}(g)=\varphi(a\varphi^{-1}(g)a^{-1})=\varphi(a)\varphi\circ\varphi^{-1}(g)\circ\varphi(a^{-1})=\varphi(a)g\varphi(a)^{-1}=\phi_{\varphi(a)}(g) \]
  which shows that $\text{Inn}(G)$ is closed under conjugation and is therefore a
  normal subgroup of $\text{Aut}(G)$.
\end{proof}


\textbf{Elaborate on why this is the case}.
The Automorphism group for $D_8$ is isomorphic to $D_8$ 

The Inner Automorphism group for $D_8$ is isomorphic to $\mathcal{K}_4$

\sk

\begin{problem}[3.4] %2
  
\end{problem}

\begin{proof}
  Let $\phi:G\rightarrow \bar{G}$ be an epimorphism with $N:=\text{ker}\phi$ and $H$ a subgroup of $G$ containing $N$. Then
  we will show that $H$ is normal in $G$ if and only if $\phi(H)$ is normal in $\bar{G}$. For the forward
  direction suppose that $H$ is normal in $G$. Let $g'\in \bar{G}$ and $h'\in \phi(H)$. Since $\phi$ is an epimorphism
  there exist $g\in G$ and $h\in H$ such that $\phi(g)=g'$ and $\phi(h)=h'$. Then
  \[ g'h'g'^{-1}=\phi(g)\phi(h)\phi(g^{-1})=\phi(ghg^{-1})\]
  which is in $\phi(H)$ since $H$ is normal. Therefore $\phi(H)$ is normal.

  Now suppose that $\phi(H)$ is normal in $\bar{G}$. Let $g\in G$ and $h\in H$. Then
  $\phi(ghg^{-1})=\phi(g)\phi(h)\phi(g^{-1})\in\phi(H)$ and since $\phi(ghg^{-1})$ lies in the image $\phi(H)$ this implies
  that $ghg^{-1}\in H$ and therefore $H$ is normal.

  Next consider the map $\varphi:H\mapsto \phi(H)$ on the lattice of subgroups containing $N$.
  We will show that it is a bijection by proving that it is surjective and
  injective. For surjectivity let $K\leq \bar{G}$. Then $\phi(K)\leq G$. Note that
  $\phi^{-1}(\bar{e})\leq\phi^{-1}(K)$ which implies that $N\leq\phi^{-1}(K)$. Therefore $\phi(\phi^{-1}(K))=K$.

  For injectivity let $\phi(H)=\phi(K)$ for $H,K\leq G$ where $H,K$ contain $N$. Without loss of generality let
  $h\in H$. Then $\phi(h)\in\phi(K)$ and $\phi(h)=\phi(k)$ for some $k\in K$. This implies that $\phi(k^{-1}h)=\bar{e}$ and
  it follows that $k^{-1}h\in N\leq K$. However since $k\in K$ we have that $h\in K$. Therefore $H\subset K$ and via the
  same reasoning $K\subset H$ and therefore $H=K$.

  Therefore the map $\varphi$ is a bijection.

  Finally let $B\subset A$ be subgroups of $G$ that contain $N$. Then define a map $C:A/B\rightarrow \phi(A)/\phi(B)$
  via $C(aB)=\phi(a)\phi(B)$. To show that the map is well defined let $aB=a'B$. Then $a=a'b$ for some $b\in B$.
  So
  \[ \phi(a)\phi(B)=\phi(a'b)\phi(B)=\phi(a')\phi(b)\phi(B)=\phi(a')\phi(B)\]
  which shows that the map $C$ is well defined.

  To show surjectivity let $a'\phi(B)\in \phi(A)/\phi(B)$. Then because $\phi$ is surjective there exists an $a\in A$ such that
  $\phi(a)=a'$. Then $C(aB)=a'\phi(B)$ which shows is surjective.

  Finally to show injectivity let $C(aB)=C(a'B)$. Then we have
  \[ \phi(a)\phi(B)=\phi(a')\phi(B)\]
  which implies that
  \[ \phi(B)=\phi(a^{-1})\phi(a')\phi(B)\]
  and thus $\phi(a^{-1}a')\in N\leq B$ which implies that $aB=a'B$.

  Therefore there is a bijection between $A/B$ and $\phi(A)/\phi(B)$ and as such $|A:B|=|\phi(A):\phi(B)|$.
\end{proof}

\sk

\begin{problem}[3.5] %3
  
\end{problem}

\begin{proof}
  Let $H$ be a normal subgroup of $G$ where $|G:H|=p$. Let $K\leq G$ then there are two cases.
  If $K\leq H$ then $K\leq H$ and we are done. Otherwise suppose that $K\nleq H$. We know that
  $|G/H|=p$ which implies that $G/H$ is cyclic. There exists a $k\in K\setminus H$ such that
  $\langle kH\rangle = G/H$. However this means that for any $g\in G$ we have $g\in k^iH$ and therefore
  $g=k^ih$ where $h\in H$. Therefore $g\in HK$ and as such $G=HK$.

  By the second isomorphsim theorem we have $G/H\cong HK/H\cong K/(H\cap K)$ which implies that
  $|K:K\cap H|=p$.
\end{proof}

\sk

\begin{problem}[3.6] %4
  
\end{problem}

\begin{proof}
  \begin{enumerate}
  \item Let $G,G'$ be groups. Then we will show that $G\times G'$ is a group
    under pointwise multiplication.

    \begin{enumerate}
    \item[associativity:] Consider elements $(a,a'),(b,b'),(c,c')\in G\times G'$.
      Then we have
      \begin{align*}
        ((a,a')\cdot(b,b'))\cdot(c,c')&=(ab,a'b')\cdot(c,c')\\
                              &=((ab)c,(a'b')c')\\
                              &= (a(bc),a'(b'c'))\\
                              &=(a,a')\cdot(bc,b'c')\\
                              &=(a,a')\cdot((b,b')\cdot(c,c'))
      \end{align*}
      Which shows that the group operation is associative.
    \item[identity:] Consider $(e,e')$ made up of the identity elements of
      $G$ and $G'$ respectively. Then for $(g,g')\in G\times G'$ we have
      \[ (e,e')\cdot(g,g')=(eg,e'g')=(g,g')=(ge,g'e')=(g,g')(e,e')\]
      which shows the existence of an identity.
    \item[inverse:] Let $(g,g')\in G$. Then 
      \begin{align*}
        (g,g')\cdot(g^{-1},g'^{-1}) &=(gg^{-1},g'g'^{-1})\\
                                &=(e,e')\\
                                &=(g^{-1}g,g'^{-1}g')\\
                                &=(g^{-1},g'^{-1})(g,g')\\
      \end{align*}
      Which shows that for any element we have a two sided inverse.
    \end{enumerate}
    Therefore the Cartesian product of groups $G\times G'$ is a group under pointwise
    multiplication.

  \item Let $M,N\trianglelefteq G$  such that $G=MN$.
  \end{enumerate}
\end{proof}

\sk

\begin{problem}[3.1.17] %5
  
\end{problem}

\begin{proof}
  
\end{proof}

\sk

\begin{problem}[3.1.32] %6
  
\end{problem}

\begin{proof}
  
\end{proof}

\sk

%%%%%%%%%%%%%%%%%%%%%%%%%%%%%%%%%%%%%%%%%%%%%%%%%%%%%%%%%%%%%%%%%%%%%%%%%%%%%
\end{document}
